src/Passes/BindToVarDecl.dfy
@@ -1,0 +1,90 @@
+include "../Interop/CSharpDafnyASTModel.dfy"
+include "../Interop/CSharpInterop.dfy"
+include "../Interop/CSharpDafnyInterop.dfy"
+include "../Interop/CSharpDafnyASTInterop.dfy"
+include "../Utils/Library.dfy"
+include "../Utils/StrTree.dfy"
+include "../Semantics/Interp.dfy"
+include "../Semantics/Equiv.dfy"
+include "../Transforms/BottomUp.dfy"
+
+module Bootstrap.Passes.BindToVarDecl {
+  // This module desugars the binds into a scope containing a var decl.
+  //
+  // TODO(SMH): we don't perform any proof for now.
+  //
+  // Ex.:
+  // ====
+  // ```
+  // let x := rhs in e
+  //
+  // ~~>
+  //
+  // {
+  //   var x := rhs;
+  //   e
+  // }
+  // ```
+
+  import Utils.Lib
+  import Utils.Lib.Debug
+  import opened Utils.Lib.Datatypes
+  import opened Transforms.BottomUp
+
+  import opened AST.Syntax
+  import opened AST.Predicates
+  import opened Semantics.Interp
+  import opened Semantics.Values
+  import opened Semantics.Equiv
+  import opened Transforms.Generic
+  import opened Transforms.Proofs.BottomUp_
+  import P = Predicates.Deep
+
+  type Expr = Syntax.Expr
+
+  function method Transform_Single(e: Expr): Expr {
+    match e {
+      case Bind(bvars, bvals, bbody) =>
+        var vdecl := Exprs.VarDecl(bvars, Exprs.Some(bvals));
+        var block := Exprs.Block([vdecl, bbody]);
+        block
+      case _ => e
+    }
+  }
+
+  predicate Tr_Pre(p: Program) {
+    true
+  }
+
+  predicate Tr_Expr_Post(e: Exprs.T) {
+    true
+  }
+
+  predicate Tr_Post(p: Program)
+  {
+    Deep.All_Program(p, Tr_Expr_Post)
+  }
+
+  const Tr_Expr : BottomUpTransformer :=
+    ( Deep.All_Expr_True_Forall(Tr_Expr_Post);
+      assume IsBottomUpTransformer(Transform_Single, Tr_Expr_Post); // TODO: prove
+      TR(Transform_Single, Tr_Expr_Post))
+
+  function method Apply_Method(m: Method) : (m': Method)
+    ensures Deep.All_Method(m', Tr_Expr_Post)
+  {
+    Deep.All_Expr_True_Forall(Tr_Expr.f.requires);
+    assert Deep.All_Method(m, Tr_Expr.f.requires);
+    Map_Method(m, Tr_Expr)
+  }
+
+  function method Apply(p: Program) : (p': Program)
+    requires Tr_Pre(p)
+    ensures Tr_Post(p')
+    // Apply the transformation to a program.
+  {
+    Deep.All_Expr_True_Forall(Tr_Expr.f.requires);
+    assert Deep.All_Program(p, Tr_Expr.f.requires);
+    Map_Program(p, Tr_Expr)
+  }
+}
